Makefile
@@ -175,11 +175,11 @@ RUSTFRONTEND=Rusttypes.v Rustsyntax.v Rustlight.v RustIR.v\
   MoveChecking.v \
   Clightgen.v Clightgenspec.v Clightgenproof.v\
   RustOp.v Rusttyping.v\
-  RustIRspec.v\
+  MapsMisc.v RustIRspec.v RustIRspecNew.v\
   BorrowCheckDomain.v ReplaceOrigins.v BorrowCheckPolonius.v\
   BorrowCheckPoloniusInterp.v\
   BorrowCheckPoloniusForward.v RegionLiveness.v\
-  MapsMisc.v BorrowCheck.v BorrowCheckInv.v BorrowCheckSound.v\
+  BorrowCheck.v BorrowCheckInv.v BorrowCheckSound.v\
   RustIRspecMem.v\
   Listmisc.v\
   BorrowCheckSim.v 
